
\title{\LaTeXe{} Template}
\date{\today}

\documentclass[12pt]{article}
\usepackage{color, soul}

\usepackage{amsmath}

\usepackage{xcolor}
\newcommand{\highlight}[1]{%
  \colorbox{yellow!50}{$\displaystyle#1$}}

\begin{document}
\maketitle

\begin{equation}
u_{p}^{l}(r, \phi) \propto r^{l} L_{p}^{l} (2r^2/w^2) e^{-r^2/w^2} \highlight{e^{-il\phi}}
\end{equation}


\begin{enumerate}
\item Low gain.
\item  $$ H \sim \int d^3\mathbf{r} \chi^{(2)}(\mathbf{r}) E_{p}^{(+)}(\mathbf{r},t) E_{s}^{(-)}(\mathbf{r},t) E_{i}^{(-)}(\mathbf{r},t)   + H.c.$$
\item  $$ H = i \hbar \Gamma \int d\mathbf{q}_{s}d\mathbf{q}_{i}F(\mathbf{q}_{s},\mathbf{q}_{i})a_{\mathbf{q}_{s}}^{\dag}a_{\mathbf{q}_{i}}^{\dag} + H.c.$$
\item  $$F(\mathbf{q}_{s},\mathbf{q}_{i}) = C\exp\big\{-\sigma^2\frac{(\mathbf{q}_{s} + \mathbf{q}_{i})^2}{2}  \big\} \textrm{sinc}\Big(\frac{L(\mathbf{q}_{s} - \mathbf{q}_{i})^2}{4k_{p}}\Big)\exp\big\{i\frac{L(\mathbf{q}_{s} - \mathbf{q}_{i})^2}{4k_{p}}\big\}  $$
\item $$ |\psi\rangle = \exp\big\{-\frac{i}{\hbar}\int_{-\infty}^{\infty} dtH(t)\big\} |0\rangle  \approx  - \frac{i}{\hbar} \int_{-\infty}^{\infty} dtH|0\rangle $$

\item Shmidt decomposition 

\item $$ F(q_{s}, q_{i}, \phi_{s} - \phi_{i}) = \sum_{n} \chi_{n}(q_{s}, q_{i})e^{in(\phi_{s} - \phi_{i})} $$

\item $$ \chi_{n}(q_{s}, q_{i}) = \sum_{m} \sqrt{\lambda_{mn}} \frac{u_{mn}(q_{s})}{\sqrt{q_{s}}} \frac{v_{mn}(q_{i})}{\sqrt{q_{i}}}   $$

\item $$ F(\mathbf{q}_{s}, \mathbf{q}_{i}) = \sum_{m,n} \sqrt{\lambda_{mn}} \frac{u_{mn}(q_{s})}{\sqrt{q_{s}}} \frac{v_{mn}(q_{i})}{\sqrt{q_{i}}} e^{in(\phi_{s} - \phi_{i})}  $$

\item broadband modes and hign gain

\item $$ A_{mn}^{\dag} = \int d\mathbf{q}_{s} \frac{u_{mn}(q_{s})}{\sqrt{q_{s}}} e^{in\phi_{s}} a_{\mathbf{q}_{s}}^{\dag} $$

\item $$ B_{mn}^{\dag} = \int d\mathbf{q}_{i} \frac{v_{mn}(q_{i})}{\sqrt{q_{i}}} e^{-in\phi_{i}} a_{\mathbf{q}_{i}}^{\dag} $$

\item $$ H = i \hbar \Gamma \sum_{m,n} \sqrt{\lambda_{mn}} (A_{mn}^{\dag} B_{mn}^{\dag} - A_{mn}B_{mn}) $$

\item $$  \frac{dA_{mn}}{dt} = \frac{i}{\hbar}[H,A_{mn}] $$ 

\item $$ A_{mn}^{out} = A_{mn}^{in}\cosh[G\sqrt{\lambda_{mn}}] + [B_{mn}^{in}]^{\dag}\sinh[G\sqrt{\lambda_{mn}}] $$

\item $$ B_{mn}^{out} = B_{mn}^{in}\cosh[G\sqrt{\lambda_{mn}}] + [A_{mn}^{in}]^{\dag}\sinh[G\sqrt{\lambda_{mn}}] $$

\item $$ \frac{d a_{\mathbf{q}_{s,i}}}{dt} = \Gamma \sum_{m,n} \sqrt{\lambda_{mn}} \frac{u_{mn}(q_{s})}{\sqrt{q_{s}}} [A_{mn}^{\dag} e^{-in\phi_{s,i}} + B_{mn}^{\dag} e^{in\phi_{s,i}}  ] $$

\item $$ \langle N_{s}(\mathbf{q}_{s}) \rangle = \sum_{m,n} \frac{|u_{mn}(q_{s})|^{2}}{q_{s}} (\sinh[G\sqrt{\lambda_{mn}}])^{2}  $$

\item three crystals

\item 
\begin{multline} 
 F(\mathbf{q}_{s},\mathbf{q}_{i}) = C\exp\big\{-\sigma^2\frac{(\mathbf{q}_{s} + \mathbf{q}_{i})^2}{2}  \big\} \textrm{sinc}\Big(\frac{\Delta \widetilde{q} L}{2}\Big) \\
 \times \Big( \exp\big\{\frac{i \Delta \widetilde{q} L}{2}\big\} +
 \exp\big\{i(\Delta \widetilde{q}^{air} d_{1} + \frac{3}{2} \Delta \widetilde{q} L) \big\} + 
 \exp\big\{i(\Delta \widetilde{q}^{air} (d_{1} + d_{2}) + \frac{5}{2} \Delta \widetilde{q} L) \big\} 
  \Big) 
\end{multline}

\item $$ \Delta\widetilde{q} = \frac{(\mathbf{q}_{s} - \mathbf{q}_{i})^2}{2k_{p}} $$

\item $$ \Delta\widetilde{q}^{air} = \frac{(\mathbf{q}_{s} - \mathbf{q}_{i})^2}{2k_{p}}n_s + \frac{2\delta n^{air}k_s}{n_s} $$


\item splitters


\begin{align*}
& |\psi_{in}\rangle = g(a_{1}^{\dag})|0\rangle  = \sum_{n=0} g_{n} (a_{1}^{\dag})^{n} |0\rangle  \\ 
& |\psi_{aux}\rangle = f(a_{2}^{\dag})|0\rangle  = \sum_{n=0} f_{n} (a_{2}^{\dag})^{n} |0\rangle  \\
& |\psi\rangle = |\psi_{in}\rangle   \otimes   |\psi_{aux}\rangle = \sum_{m,n} \alpha_{m,n} (a_{1}^{\dag})^{m} (a_{2}^{\dag})^{n} |0\rangle^{\otimes 2} \\
& \sum_{m,n} |\alpha_{m,n}|^2 = 1 
\end{align*}

\item loseless BS

\item $$ \sum_{m,n} |\alpha_{m,n}|^2 = 1 $$

\item $$ \sum_{m,n} |\alpha_{m,n}^{(2)}|^2 = 1 $$

\begin{align*}
&  r_{j}^2 + t_{j}^2 + a_{j}^2 = 1 \\
&  a_{1}^{\dag} \rightarrow  r_{j}a_{1}^{\dag} + it_{j}a_{2}^{\dag} \\
&  a_{2}^{\dag} \rightarrow  r_{j}a_{2}^{\dag} + it_{j}a_{1}^{\dag} 
\end{align*}


\item state in area 2 after first BS

\item $$ |\psi_{2}\rangle = \sum_{m,n} \alpha_{m,n}^{(2)} (a_{1}^{\dag})^{m} (a_{2}^{\dag})^{n} |0\rangle^{\otimes 2}  $$

\item 4 channels

\item $$ |\psi_3\rangle = \sum_{p_{1},p_{2},p_{3},p_{4}} \beta_{p_{1},p_{2},p_{3},p_{4}} (a_{1}^{\dag})^{p_{1}} (a_{2}^{\dag})^{p_{2}} (a_{3}^{\dag})^{p_{3}} (a_{4}^{\dag})^{p_{4}} |0\rangle^{\otimes 4}  $$


\item First and only one ideal detector was clicked

\item $$ |\psi_4\rangle = \sum_{\substack{p_{1},p_{2},p_{4} \\ p_{1} > 0, p_{3}=0}} |\beta_{p_{1},p_{2},0,p_{4}} \sqrt{p_{1}!p_{2}!p_{4}!}|^2 |p_{2}, p_{4}\rangle $$

\item First and third detectors were clicked

\item $$ |\psi_4\rangle = \sum_{\substack{p_{1},p_{2},p_{3},p_{4} \\ p_{1} > 0, p_{3}>0}} |\beta_{p_{1},p_{2},p_{3},p_{4}} \sqrt{p_{1}!p_{2}!p_{3}!p_{4}!}|^2 |p_{2}, p_{4}\rangle $$

\item No detection

\item $$ |\psi_4\rangle = \sum_{\substack{p_{2},p_{4} \\ p_{1}=0, p_{3}=0}} |\beta_{0,p_{2},0,p_{4}} \sqrt{p_{2}!p_{4}!}|^2 |p_{2}, p_{4}\rangle $$



\item final state

\item $$ |\psi_{out}\rangle = \sum_{m,n} \alpha_{m,n}^{out} (a_{1}^{\dag})^{m} (a_{2}^{\dag})^{n} |0\rangle^{\otimes 2}  $$

\item example with two coherent states - alpha=1

\item $$ |\psi\rangle = |\alpha\rangle \otimes |\alpha\rangle, \quad \alpha = 1 $$


\item two coherent after BS
\item $$ |\psi_{2}\rangle \approx  e^{-1} (1 + \frac{1 + i}{\sqrt{2}}a_{1}^{\dag} + \frac{1 + i}{\sqrt{2}}a_{2}^{\dag} + ia_{1}^{\dag}a_{2}^{\dag} + \frac{i}{2}(a_{1}^{\dag})^{2} + \frac{i}{2}(a_{2}^{\dag})^{2} + \frac{i - 1}{2\sqrt{2}}a_{1}^{\dag}(a_{2}^{\dag})^{2} + \frac{i - 1}{2\sqrt{2}}(a_{1}^{\dag})^{2}a_{2}^{\dag} + ... ) $$


\item auto correlation
\begin{equation*}
	\begin{aligned}
	Autocorr_{s}(q, q^{'}) = \langle N_s(q)N_s(q^{'}) \rangle -  \langle N_s(q) \rangle \langle N_s(q^{'})\rangle = \\
	= \langle a_{s}^{\dag}(q)a_{s}(q)a_{s}^{\dag}(q^{'})a_{s}(q^{'}) \rangle  -  \langle a_{s}^{\dag}(q)a_{s}(q) \rangle \langle a_{s}^{\dag}(q^{'})a_{s}(q^{'}) \rangle
	\end{aligned}
\end{equation*}


\item cross correlation
\begin{equation*}
	\begin{aligned}
	Crosscorr(q, q^{'}) = \langle N_s(q)N_i(q^{'}) \rangle -  \langle N_s(q) \rangle \langle N_i(q^{'}) \rangle = \\
	= \langle a_{s}^{\dag}(q)a_{s}(q)a_{i}^{\dag}(q^{'})a_{i}(q^{'}) \rangle  -  \langle a_{s}^{\dag}(q)a_{s}(q) \rangle \langle a_{i}^{\dag}(q^{'})a_{i}(q^{'}) \rangle
	\end{aligned}
\end{equation*}


\item POVM operators.

\begin{align*}
&  \Pi_{no-click} = \sum_{n=0}^{\infty} (1-\eta_{SPD})^n  |n\rangle  \langle n|   \\
&  \Pi_{click} = 1 - \Pi_{no-click} = \sum_{n=0}^{\infty}[1 - (1-\eta_{SPD})^n]  |n\rangle  \langle n|
\end{align*}




\item After projection

\item Only first clicked
\item $$ |\psi_{out}\rangle = \Pi_{click}^{(1)} |\psi_{in}\rangle $$

\item Two clicked 1st and 3rd
\item $$ |\psi_{out}\rangle = \Pi_{click}^{(1)}\Pi_{click}^{(3)}  |\psi_{in}\rangle $$



\item First and only one ideal detector was clicked

\item $$ |\psi_4\rangle = \sum_{\substack{p_{1},p_{2},p_{4} \\ p_{1} \neq 0, p_{3}=0}} \beta_{p_{1},p_{2},0,p_{4}} \sqrt{p_{1}!} (b_{2}^{\dag})^{p_{2}} (b_{4}^{\dag})^{p_{4}}  |0\rangle^{\otimes 2} $$

\item First and third detectors were clicked

\item $$ |\psi_4\rangle = \sum_{\substack{p_{1},p_{2},p_{3},p_{4} \\ p_{1} \neq 0, p_{3} \neq 0}} \beta_{p_{1},p_{2},p_{3},p_{4}} \sqrt{p_{1}!p_{3}!} (b_{2}^{\dag})^{p_{2}} (b_{4}^{\dag})^{p_{4}} |0\rangle^{\otimes 2} $$

\item No detection

\item $$ |\psi_4\rangle = \sum_{\substack{p_{2},p_{4} \\ p_{1}=0, p_{3}=0}} \beta_{0,p_{2},0,p_{4}} (b_{2}^{\dag})^{p_{2}} (b_{4}^{\dag})^{p_{4}} |0\rangle^{\otimes 2} $$

\item Projection operators




\item It starts here 


\item States.

\begin{align*}
& |\psi_{in}\rangle = g(a_{1}^{\dag})|0\rangle  = \sum_{n=0} g_{n} (a_{1}^{\dag})^{n} |0\rangle  \\ 
& |\psi_{aux}\rangle = f(a_{2}^{\dag})|0\rangle  = \sum_{n=0} f_{n} (a_{2}^{\dag})^{n} |0\rangle  \\
& |\psi\rangle = |\psi_{in}\rangle   \otimes   |\psi_{aux}\rangle = \sum_{m,n} \alpha_{m,n} (a_{1}^{\dag})^{m} (a_{2}^{\dag})^{n} |0\rangle^{\otimes 2} \\
& \sum_{m,n} |\alpha_{m,n}|^2 = 1 
\end{align*}

\item Beam splitter.

\begin{align*}
&  r_{j}^2 + t_{j}^2 + a_{j}^2 = 1 \\
&  a_{1}^{\dag} \rightarrow  r_{j}a_{1}^{\dag} + it_{j}a_{2}^{\dag} \\
&  a_{2}^{\dag} \rightarrow  r_{j}a_{2}^{\dag} + it_{j}a_{1}^{\dag} 
\end{align*}


\item POVM operators.

\begin{align*}
&  \Pi_{no-click} = \sum_{n=0}^{\infty} (1-\eta_{SPD})^n  |n\rangle  \langle n|   \\
&  \Pi_{click} = 1 - \Pi_{no-click} = \sum_{n=0}^{\infty}[1 - (1-\eta_{SPD})^n]  |n\rangle  \langle n|
\end{align*}



\begin{align*} 
&  \hat{\Pi} = \Pi_{click}^{(1)} \otimes  \textrm{I}^{(2)}  \otimes  \Pi_{click}^{(3)} \otimes  \textrm{I}^{(4)}   \\
&  \hat{\Pi} = \Pi_{click}^{(1)} \otimes  \textrm{I}^{(2)}  \otimes  \Pi_{no-click}^{(3)} \otimes  \textrm{I}^{(4)}  \\ 
&  \hat{\Pi} = \Pi_{no-click}^{(1)} \otimes  \textrm{I}^{(2)}  \otimes  \Pi_{click}^{(3)} \otimes  \textrm{I}^{(4)} \\
&    \hat{\Pi} = \Pi_{no-click}^{(1)} \otimes  \textrm{I}^{(2)}  \otimes  \Pi_{no-click}^{(3)} \otimes  \textrm{I}^{(4)}  
\end{align*}

\item State before detection.

\item $$ |\psi_4\rangle = \sum_{p_{1},p_{2},p_{3},p_{4}} \beta_{p_{1},p_{2},p_{3},p_{4}} (b_{1}^{\dag})^{p_{1}}  (b_{2}^{\dag})^{p_{2}} (b_{3}^{\dag})^{p_{3}}  (b_{4}^{\dag})^{p_{4}} |0\rangle^{\otimes 4} $$

\item Detection.

\item $$  \rho =  Tr_{1,3}(\hat{\Pi} |\psi_{in}\rangle \langle \psi_{in}|   \hat{\Pi}^{\dag}) $$


\item dens matrix after detection

\item $$ \rho = \sum_{\substack{p_{2},p_{4} \\ p'_{2}, p'_{4}}}  \rho_{p_{2},p_{4}, p'_{2}, p'_{4}} |p_{2}\rangle \langle p'_{2}| \otimes |p_{4}\rangle \langle p'_{4}| $$

\item Last BS:

\item $$   |p_{2},p_{4}\rangle \langle p'_{2},p'_{4}| = \frac{1}{\sqrt{p_{2}!p_{4}!p'_{2}!p'_{4}!}} (a_{2}^{\dag})^{p_{2}} (a_{4}^{\dag})^{p_{4}} |0,0\rangle \langle 0,0| (a_{2})^{p'_{2}} (a_{4})^{p'_{4}}   $$


\item Density matrix after detection.

\item $$ \rho^{out} = \sum_{\substack{p_{1},p_{2} \\ p'_{1}, p'_{2}}}  \rho^{out}_{p_{1},p_{2}, p'_{1}, p'_{2}} |p_{1}\rangle \langle p'_{1}| \otimes |p_{2}\rangle \langle p'_{2}| $$

\item Density matrix of subsystem.

\item $$ \rho_{1} = Tr_{2}(\rho_{12}) $$

\item Von Neumann entropy.

\begin{align*}
& S(\rho_{12}) = - \sum_{n} \lambda_{n} \ln(\lambda_{n})  \\
& \rho_{1}   \rightarrow  \{ \lambda_{n} \}, \ eigenvalues 
\end{align*}

\item Linear entropy.
\item $$ S_{L}(\rho_{12}) =  1 - Tr(\rho_{1}^2) $$

\item Negativity.
\begin{align*}
& N(\rho) = \frac{||\rho^{T_{1}}||_{1} - 1}{2}  =\sum_{n}  \frac{|\lambda_{n}| - \lambda_{n}}{2} \\
& \rho_{12}   \rightarrow  \{ \lambda_{n} \}, \ eigenvalues  \\
\\
& LN(\rho) := \log_{2}(2N + 1)
\end{align*}


\end{enumerate}


\end{document}